Added specifications for producer/consumer

theories/examples/producer_consumer.v
@@ -6,6 +6,7 @@ From iris.heap_lang.lib Require Import spin_lock.
 From osiris.utils Require Import list compare.
 
 
+Definition qnew : val := λ: <>, #().
 Definition qenqueue : val := λ: "q" "v", #().
 Definition qdequeue : val := λ: "q", #().
 Definition qis_empty : val := λ: "q", #().
@@ -36,6 +37,7 @@ Definition dist_queue : val :=
 
 Definition producer : val :=
   rec: "go" "c" "l" "produce" :=
+    (* acquire "l";; *)
     match: "produce" #() with
       SOME "v" =>
         acquire "l";;
@@ -47,15 +49,86 @@ Definition producer : val :=
         send "c" #enq;; send "c" #stop
         release "l"
     end.
-        
+
 Definition consumer : val :=
   rec: "go" "c" "l" "consume" :=
     acquire "l";;
     send "c" #deq;;
     if: recv "c"             (* cont/stop *)
     then if: recv "c"        (* some/none *)
-         then let: "v" := recv "c" in
-              release "l";; "produce" "v";; "go" "c" "l" "consume"
+         then let: "v" := SOME (recv "c") in
+              release "l";; "consume" "v";; "go" "c" "l" "consume"
+              (* "consume" "v";; release "l";; "go" "c" "l" "consume" *)
          else release "l";; "go" "c" "l" "consume"
-    else release "l";; #().
+    else "consume" NONE;; release "l";; #().
+    (* else release "l";; "consume" NONE;; #(). *)
 
+(* Makes n producers and m consumers *)
+Definition produce_consume : val :=
+  λ: "produce" "consume" "pc" "cc",
+  #().
+
+Section list_sort_elem.
+  Context `{!heapG Σ, !proto_chanG Σ} (N : namespace).
+
+  Definition queue_prot : iProto Σ := (END)%proto.
+
+  Lemma dist_queue_spec c :
+    {{{ c ↣ queue_prot @ N }}}
+      dist_queue (qnew #()) #0 #0 c
+    {{{ RET #(); c ↣ END @ N }}}.
+  Proof. Admitted.
+
+  (* Need predicate for end of production? *)
+  Definition produce_spec σ P (produce : val) :=
+    ∀ vs,
+    {{{ σ vs }}}
+      produce #()
+    {{{ v, RET v; (∃ w, ⌜v = SOMEV w⌝ ∧ P w ∗ σ (w::vs)) ∨ (⌜v = NONEV⌝) }}}.
+
+  Definition consume_spec σ P Q (consume : val) :=
+    ∀ vs, ∀ v : val,
+    {{{ σ vs ∗ P v }}}
+      consume v
+    {{{ RET #(); σ (v::vs) ∗ Q v }}}.
+
+  Lemma produce_consume_spec produce consume pσ cσ P Q pc cc :
+    pc > 0 → cc > 0 → 
+    produce_spec pσ P produce →
+    consume_spec cσ P Q consume →
+    {{{ pσ [] ∗ cσ [] }}}
+      produce_consume produce consume #pc #cc
+    {{{ vs, RET #(); pσ vs ∗ cσ vs ∗ [∗ list] v ∈ vs, Q v }}}.
+  Proof. Admitted.
+
+  (* Example producer *)
+  Definition ints_to_n (l : val) (n:nat) : val:=
+    λ: <>, let: "v" := !l in
+           if: "v" < #n
+           then l <- "v" + #1;; SOME "v"
+           else NONE.
+
+  Lemma ints_to_n_spec l n :
+    produce_spec (λ vs, (∃ loc, ⌜loc = LitV $ LitLoc l⌝ ∗ l ↦ #(length vs))%I)
+                 (λ v, ⌜∃ i, v = LitV $ LitInt i⌝%I) (ints_to_n #l n).
+  Proof.
+    iIntros (vs Φ) "Hσ HΦ".
+    iDestruct "Hσ" as (loc ->) "Hσ".
+    wp_lam. wp_load. wp_pures.
+    case_bool_decide.
+    - wp_store. wp_pures. iApply "HΦ".
+      (* Does this not exist? *)
+      assert (∀ n : nat, (n + 1) = (S n)). intros m. lia. rewrite H0.
+      by eauto 10 with iFrame.
+    - wp_pures. iApply "HΦ". by iRight.
+  Qed.
+
+  Definition consume_to_list l : val:=
+    λ: "v", 
+      let: "xs" := !l in
+      l <- lcons "v" "xs".
+
+  Lemma consume_to_list_spec l :
+    consume_spec (λ vs, (∃ loc, ⌜loc = LitV $ LitLoc l⌝ ∗ l ↦ val_encode vs)%I)
+                 (λ v, ⌜True⌝%I) (λ v, ⌜True⌝%I) (consume_to_list #l).
+  Proof. Admitted.
